`Server.Audit` spec (- keys). Audit proof as tying down new digs from prevDig

new/proof/github_com/sanjit_bhat/pav/ktcore_proof/ktcore.v
@@ -340,9 +340,9 @@ Definition wish_NonMemb pk uid ver dig nonMemb : iProp Σ :=
   "#His_vrf_out" ∷ cryptoffi.is_vrf_out pk enc label ∗
   "#Hwish_nonMemb" ∷ merkle.wish_NonMemb label nonMemb.(ktcore.NonMemb.MerkleProof) dig.
 
-Definition wish_ListUpdate updates digs : iProp Σ :=
-  "%Hlen" ∷ ⌜length digs = if decide (length updates = 0%nat)
-    then 0%nat else S (length updates)⌝ ∗
+Definition wish_ListUpdate_aux prevDig updates digs : iProp Σ :=
+  "%Hlen" ∷ ⌜length digs = S (length updates)⌝ ∗
+  "%Hhead" ∷ ⌜head digs = Some prevDig⌝ ∗
   "#Hwish_updates" ∷ ([∗ list] i ↦ upd ∈ updates,
     ∃ dig0 dig1,
     "%Hlook0" ∷ ⌜digs !! i = Some dig0⌝ ∗
@@ -351,15 +351,13 @@ Definition wish_ListUpdate updates digs : iProp Σ :=
       upd.(ktcore.UpdateProof.MapVal) upd.(ktcore.UpdateProof.NonMembProof)
       dig0 dig1).
 
-Lemma wish_ListUpdate_det updates digs0 digs1 :
-  wish_ListUpdate updates digs0 -∗
-  wish_ListUpdate updates digs1 -∗
+Lemma wish_ListUpdate_aux_det prevDig updates digs0 digs1 :
+  wish_ListUpdate_aux prevDig updates digs0 -∗
+  wish_ListUpdate_aux prevDig updates digs1 -∗
   ⌜digs0 = digs1⌝.
 Proof.
   iNamedSuffix 1 "0".
   iNamedSuffix 1 "1".
-  case_decide.
-  { by destruct digs0, digs1. }
   (* no way to apply [list_eq_same_length] directly. *)
   iAssert (⌜∀ (i : nat) x y,
     digs0 !! i = Some x → digs1 !! i = Some y → x = y⌝)%I as %?.
@@ -367,20 +365,86 @@ Proof.
   iIntros (i ?? Hlook0 Hlook1).
   apply lookup_lt_Some in Hlook0 as ?.
   destruct i.
-  - list_elem updates 0%nat as upd.
-    iDestruct (big_sepL_lookup with "Hwish_updates0") as "{Hwish_updates0} H0"; [done|].
-    iDestruct (big_sepL_lookup with "Hwish_updates1") as "{Hwish_updates1} H1"; [done|].
-    iNamedSuffix "H0" "0".
-    iNamedSuffix "H1" "1".
-    simplify_eq/=.
-    by iDestruct (merkle.wish_Update_det with "Hwish0 Hwish1") as %[-> ->].
-  - list_elem updates i as upd.
-    iDestruct (big_sepL_lookup with "Hwish_updates0") as "{Hwish_updates0} H0"; [done|].
-    iDestruct (big_sepL_lookup with "Hwish_updates1") as "{Hwish_updates1} H1"; [done|].
-    iNamedSuffix "H0" "0".
-    iNamedSuffix "H1" "1".
-    simplify_eq/=.
-    by iDestruct (merkle.wish_Update_det with "Hwish0 Hwish1") as %[-> ->].
+  { iPureIntro.
+    rewrite !head_lookup in Hhead0, Hhead1.
+    by simplify_eq/=. }
+  list_elem updates i as upd.
+  iDestruct (big_sepL_lookup with "Hwish_updates0") as "H0"; [done|].
+  iDestruct (big_sepL_lookup with "Hwish_updates1") as "H1"; [done|].
+  iNamedSuffix "H0" "0".
+  iNamedSuffix "H1" "1".
+  simplify_eq/=.
+  by iDestruct (merkle.wish_Update_det with "Hwish0 Hwish1") as %[-> ->].
+Qed.
+
+Definition wish_ListUpdate prevDig updates nextDig : iProp Σ :=
+  ∃ digs,
+  "#Hwish_aux" ∷ wish_ListUpdate_aux prevDig updates digs ∗
+  "%Hlast" ∷ ⌜last digs = Some nextDig⌝.
+
+Lemma wish_ListUpdate_det prevDig updates nextDig0 nextDig1 :
+  wish_ListUpdate prevDig updates nextDig0 -∗
+  wish_ListUpdate prevDig updates nextDig1 -∗
+  ⌜nextDig0 = nextDig1⌝.
+Proof.
+  iNamedSuffix 1 "0".
+  iNamedSuffix 1 "1".
+  iDestruct (wish_ListUpdate_aux_det with "Hwish_aux0 Hwish_aux1") as %->.
+  rewrite Hlast0 in Hlast1.
+  by simplify_eq/=.
+Qed.
+
+Definition wish_ListAudit prevDig audits digs : iProp Σ :=
+  "%Hlen" ∷ ⌜length digs = S (length audits)⌝ ∗
+  "%Hhead" ∷ ⌜head digs = Some prevDig⌝ ∗
+  "#Hwish_audits" ∷ ([∗ list] i ↦ aud ∈ audits,
+    ∃ dig0 dig1,
+    "%Hlook0" ∷ ⌜digs !! i = Some dig0⌝ ∗
+    "%Hlook1" ∷ ⌜digs !! (S i) = Some dig1⌝ ∗
+    "#Hwish" ∷ wish_ListUpdate dig0 aud.(AuditProof.Updates) dig1).
+
+Lemma wish_ListAudit_det prevDig audits digs0 digs1 :
+  wish_ListAudit prevDig audits digs0 -∗
+  wish_ListAudit prevDig audits digs1 -∗
+  ⌜digs0 = digs1⌝.
+Proof.
+  iNamedSuffix 1 "0".
+  iNamedSuffix 1 "1".
+  iInduction audits as [] using rev_ind forall (digs0 digs1 Hlen0 Hlen1 Hhead0 Hhead1).
+  { destruct digs0, digs1; try done.
+    destruct digs0, digs1; try done.
+    by simplify_eq/=. }
+  destruct digs0 using rev_ind; try done. clear IHdigs0.
+  destruct digs1 using rev_ind; try done. clear IHdigs1.
+  autorewrite with len in *.
+  iDestruct (big_sepL_snoc with "Hwish_audits0") as "{Hwish_audits0} (Hwish_aud0&H0)".
+  iDestruct (big_sepL_snoc with "Hwish_audits1") as "{Hwish_audits1} (Hwish_aud1&H1)".
+  iNamedSuffix "H0" "0".
+  iNamedSuffix "H1" "1".
+  iDestruct ("IHaudits" $! digs0 digs1 with "[][][][][][]") as %->;
+    iClear "IHaudits".
+  1-4: iPureIntro.
+  1-2: lia.
+  { by destruct digs0. }
+  { by destruct digs1. }
+  { iModIntro. iApply (big_sepL_impl with "Hwish_aud0"). iModIntro.
+    iIntros (?? Hlook) "@".
+    apply lookup_lt_Some in Hlook.
+    rewrite !lookup_app_l in Hlook0, Hlook1; [|lia..].
+    iFrame "#%". }
+  { iModIntro. iApply (big_sepL_impl with "Hwish_aud1"). iModIntro.
+    iIntros (?? Hlook) "@".
+    apply lookup_lt_Some in Hlook.
+    rewrite !lookup_app_l in Hlook0, Hlook1; [|lia..].
+    iFrame "#%". }
+  iClear "Hwish_aud0 Hwish_aud1".
+  simplify_eq/=.
+  rewrite !lookup_app_l in Hlook00, Hlook01; [|lia..].
+  rewrite !lookup_app_r in Hlook10, Hlook11; [|lia..].
+  apply list_lookup_singleton_Some in Hlook10 as [_ ->].
+  apply list_lookup_singleton_Some in Hlook11 as [_ ->].
+  simplify_eq/=.
+  by iDestruct (wish_ListUpdate_det with "Hwish0 Hwish1") as %->.
 Qed.
 
 End proof.
